$$
\begin{align}
e^x&=1+x+\frac{x^2}{2 !}+\frac{x^3}{3 !}+\frac{x^4}{4 !}+\ldots\\
&\downarrow\\
e^{i x}&=1+i x+\frac{(i x)^2}{2 !}+\frac{(i x)^3}{3 !}+\frac{(i x)^4}{4 !}+\ldots\\
&\downarrow\\
e^{i x} &=1+i x+\frac{x^2}{2 !}+\frac{i x^3}{3 !}+\frac{x^4}{4 !}+\frac{i x^5}{5 !}+\ldots\\
&\downarrow\\
e^{i x}&=1+i\left(x-\frac{x^3}{3 !}+\frac{x^5}{5 !}+\cdots\right)-\frac{x^2}{2 !}+\frac{x^4}{4 !} \cdots\\
&\downarrow\\
e^{i x}&=\cos (x)+i \sin (x)\\
&\downarrow\\
e^{i \pi}&=\cos (\pi)+i \sin (\pi)\\
&\downarrow\\
e^{i \pi}&=-1\\
&\downarrow\\
e^{i \pi} + 1&= 0\\
\end{align}
$$
